\documentclass{article}
\usepackage{ifthen}
\usepackage{epsfig}
\usepackage[utf8]{inputenc}
\usepackage{newunicodechar}
  \newunicodechar{⁻}{${}^{-}$}% Superscript minus
  \newunicodechar{²}{${}^{2}$}% Superscript two
  \newunicodechar{³}{${}^{3}$}% Superscript three

\pagestyle{empty}
\begin{document}
$ \frac{\partial \rho}{\partial t} + \nabla \cdot (\rho u) = S(x,t) $
\pagebreak

$ \nabla \cdot (\rho \gamma u Q)$
\pagebreak

$\gamma$
\pagebreak

$Q$
\pagebreak

$ \nabla \cdot (\rho u Q)$
\pagebreak

$N = \nabla \cdot (u \rho \gamma Q)$
\pagebreak

$\rho$
\pagebreak

$ Q $
\pagebreak

$ \kappa $
\pagebreak

$ \lambda $
\pagebreak

$ F $
\pagebreak

\[ \frac{dQ}{dt} + (\vec{u}^{\mbox{\scriptsize ADV}} \cdot \nabla)Q = F, \]
\pagebreak

$\vec{u}^{\mbox{\scriptsize ADV}}$
\pagebreak

$F$
\pagebreak

\[ \frac{dQ}{dt} + \nabla \cdot (\vec{u}^{\mbox{\scriptsize ADV}} Q) = F. \]
\pagebreak

$\vec{u}$
\pagebreak

$ \vec{N}^{n+\frac{1}{2}} = \vec{u}^{\mbox{\scriptsize ADV},n+\frac{1}{2}} \cdot \nabla q^{n+\frac{1}{2}} $
\pagebreak

$ \vec{f} $
\pagebreak

$ q $
\pagebreak

$ \vec{u}^{\mbox{\scriptsize ADV}} $
\pagebreak

\begin{eqnarray*} f_{i+\frac{1}{2},j,k}^{n+\frac{1}{2}} &=& \Delta t \, *u_{i+\frac{1}{2},j,k}^{\mbox{\scriptsize ADV},n+\frac{1}{2}} \, *q_{i+\frac{1}{2},j,k}^{n+\frac{1}{2}} \\ f_{i,j+\frac{1}{2},k}^{n+\frac{1}{2}} &=& \Delta t \, *v_{i,j+\frac{1}{2},k}^{\mbox{\scriptsize ADV},n+\frac{1}{2}} \, *q_{i,j+\frac{1}{2},k}^{n+\frac{1}{2}} \\ f_{i,j,k+\frac{1}{2}}^{n+\frac{1}{2}} &=& \Delta t \, *w_{i,j,k+\frac{1}{2}}^{\mbox{\scriptsize ADV},n+\frac{1}{2}} \, *q_{i,j,k+\frac{1}{2}}^{n+\frac{1}{2}} \end{eqnarray*}
\pagebreak

$ \vec{u}^{\mbox{\scriptsize ADV}} = (u^{\mbox{\scriptsize ADV}},v^{\mbox{\scriptsize ADV}},w^{\mbox{\scriptsize ADV}}) $
\pagebreak

\[ \frac{dQ}{dt} + (\vec{u}^{\mbox{\scriptsize ADV}} \cdot \nabla)Q = 0, \]
\pagebreak

$ \vec{V} $
\pagebreak

\[ \frac{d\vec{V}}{dt} + (\vec{u}^{\mbox{\scriptsize ADV}} \cdot \nabla)\vec{V} = 0, \]
\pagebreak

\[ \frac{d\vec{V}}{dt} + (\vec{u}^{\mbox{\scriptsize ADV}} \cdot \nabla)\vec{V} = *\vec{F}, \]
\pagebreak

\[ \frac{dQ}{dt} + \nabla \cdot (\vec{u}^{\mbox{\scriptsize ADV}} Q) = F - Q \nabla \cdot *\vec{u}^{\mbox{\scriptsize ADV}}, \]
\pagebreak

\[ \frac{dQ}{dt} + (\vec{u}^{\mbox{\scriptsize ADV}} \cdot \nabla) Q = F. \]
\pagebreak

$ [t^{n+1}, t^n] $
\pagebreak

$ \zeta q + \kappa n \dot \nabla q = \g $
\pagebreak

$ n \dot B = g $
\pagebreak

$ \nabla \dot (\chi B) - \chi \nabla \dot B $
\pagebreak

$\lambda$
\pagebreak

$ C = \sum_{Dirichlet} \chi_i/\eta + \sum_{Robin} \nabla \dot (\chi_i n_i) - \chi_i \nabla \dot n_i$
\pagebreak

$\chi_i = 1-H_i$
\pagebreak

$ D = \kappa + \sum_{Neumann} (-\chi_i + \eta \chi_i) + \sum_{Robin} (-\chi_i + \eta \chi_i)$
\pagebreak

$ F_i = \chi_i/\eta Q_{bc}$
\pagebreak

$ F_i = \nabla \dot (\chi_i B) - \chi_i \nabla \dot B_i $
\pagebreak

$B_i$
\pagebreak

$F = \sum_{i} F_i$
\pagebreak

$ u \dot \grad Q$
\pagebreak

$ N = (1-\sum_{Neumann and Robin} \chi_i) N$
\pagebreak

$ \vec{\lambda}$
\pagebreak

$ \vec{U}$
\pagebreak

\begin{eqnarray*} \beta J L^{-1} S \gamma \vec{\lambda} &=& M \vec{\lambda} = \vec{w} \\ T M T^* \vec{U} &=& \vec{F}. \end{eqnarray*}
\pagebreak

$ J $
\pagebreak

$ S $
\pagebreak

$ L $
\pagebreak

$ T $
\pagebreak

$ \vec{w} $
\pagebreak

$ \vec{F} $
\pagebreak

$ \vec{v} $
\pagebreak

$ p $
\pagebreak

$ \vec{\lambda} $
\pagebreak

$ \vec{U} $
\pagebreak

\begin{eqnarray*} A \vec{v} + \nabla p - \gamma S \vec{\lambda} &=& \vec{g} \\ -\nabla \cdot \vec{v} &=& (h = 0) \\ -\beta J \vec{v} + \beta T^{*} \vec{U} -\beta \delta \vec{\lambda} &=& (\vec{w} = -\beta \vec{U}_{\mbox{\scriptsize def}}) \\ T \vec{\lambda} &=& \vec{F} \end{eqnarray*}
\pagebreak

\begin{eqnarray*} A \vec{v} + \nabla p - \gamma S \vec{\lambda} &=& \vec{g} \\ -\nabla \cdot \vec{v} &=& (h = 0) \\ -\beta J \vec{v} - \beta \delta \vec{\lambda} &=& (w = -\beta (T^{*}\vec{U}+ \vec{U}_{\mbox{\scriptsize def}}) = -\beta \vec{U}_{\mbox{\scriptsize imposed}}) \end{eqnarray*}
\pagebreak

$ A $
\pagebreak

$ G $
\pagebreak

$ T^{*} $
\pagebreak

$ \vec{U}_{\mbox{\scriptsize def}} $
\pagebreak

$ \vec{U}_{\mbox{\scriptsize imposed}} $
\pagebreak

$ \gamma $
\pagebreak

$ \beta $
\pagebreak

$ \delta $
\pagebreak

$Ax=b$
\pagebreak

$x$
\pagebreak

$y=Ax$
\pagebreak

$[u,v,\omega_z]$
\pagebreak

$[u,v,w,\omega_x,\omega_y,\omega_z]$
\pagebreak

$ U_{sub} \leq NDIM * (NDIM + 1) / 2 $
\pagebreak

$ U_{sub} = NDIM * (NDIM + 1) / 2 $
\pagebreak

$ = \alpha * mobility_mat + \beta * identity_mat. $
\pagebreak

$ \theta_n = \theta_{n-1} + \omega_{n-1} \triangle t $
\pagebreak

$ \phi $
\pagebreak

$y=F[x]$
\pagebreak

$ [MM] = \alpha*[MM] + \beta*[I]. $
\pagebreak

$ |\nabla Q | = 1 $
\pagebreak

$ \phi(s) = \partial \Omega $
\pagebreak

$ k $
\pagebreak

$ l $
\pagebreak

\[ \vec{F}_k = \kappa_{k,l} \left( \|\vec{X}_{l} - \vec{X}_{k}\| - r_{k,l} \right) *\frac{\vec{X}_{l} - \vec{X}_{k}}{\|\vec{X}_{l} - \vec{X}_{k}\|}, \]
\pagebreak

\[ \vec{F}_l = \kappa_{k,l} \left( \|\vec{X}_{l} - \vec{X}_{k}\| - r_{k,l} \right) *\frac{\vec{X}_{k} - \vec{X}_{l}}{\|\vec{X}_{l} - \vec{X}_{k}\|} = - \vec{F}_k, \]
\pagebreak

$ \kappa_{k,l} $
\pagebreak

$ r_{k,l} $
\pagebreak

$ T_{k,l} $
\pagebreak

\[ T_{k,l} = \kappa_{k,l} \left( \|\vec{X}_{l} - \vec{X}_{k}\| - r_{k,l} \right). \]
\pagebreak

\[ \vec{F}_k = T_{k,l} \frac{\vec{X}_{l} - \vec{X}_{k}}{\|\vec{X}_{l} - \vec{X}_{k}\|} \]
\pagebreak

\[ \vec{F}_l = T_{k,l} \frac{\vec{X}_{k} - \vec{X}_{l}}{\|\vec{X}_{k} - \vec{X}_{l}\|}. \]
\pagebreak

$ \eta $
\pagebreak

$ b = (1-a) $
\pagebreak

$a$
\pagebreak

$b$
\pagebreak

$ a\mathbf{u} + b\tau\cdot\mathbf{n} = \mathbf{g}$
\pagebreak

$\tau = -p\mathbf{I} + \frac{\mu}{2}\left(\nabla\mathbf{u} + \nabla\mathbf{u}^T\right)$
\pagebreak

$\mu$
\pagebreak

$ a$
\pagebreak

$ b $
\pagebreak

$ a = 1 $
\pagebreak

$b = 1$
\pagebreak

$a + b = 1$
\pagebreak

$ \nabla \cdot \mathbf{u} $
\pagebreak

$ \nabla \cdot \mathbf{u} = 0 $
\pagebreak

$(\frac{\partial \rho u}{\partial t} + N(\rho u)) = -\nabla p + \nabla \cdot \mu (\nabla u) + (\nabla u)^T )$
\pagebreak

$ N(u) = \nabla \cdot (\rho u u) $
\pagebreak

$ \frac{\partial \rho}{\partial t} + \nabla \cdot (\rho u) = 0 $
\pagebreak

$\rho^n$
\pagebreak

$\rho^{n+\frac{1}{2}}$
\pagebreak

$N(\rho u)$
\pagebreak

$\rho^{n+1}$
\pagebreak

$ \nabla \cdot (\rho u u)$
\pagebreak

$ S(x,t) $
\pagebreak

$N = \nabla \cdot (u \rho u)$
\pagebreak

$ c A + G(c x_p) = c b_u$
\pagebreak

$ c $
\pagebreak

$ c(\frac{\rho}{dt} - \frac{\mu}{dx^2}) \sim \frac{1}{dx} $
\pagebreak

$ (\nabla \cdot) \sim \frac{1}{dx} $
\pagebreak

$ dt \sim dx $
\pagebreak

$ 1/dx = N $
\pagebreak

$ c \sim \frac{1}{\rho - \mu N} $
\pagebreak

$ N $
\pagebreak

$ dx $
\pagebreak

$ \nabla \cdot \mathbf{u} = Q $
\pagebreak

$ t = 0 $
\pagebreak

$ Q = 0 $
\pagebreak

$\rho(\frac{\partial u}{\partial t} + N(u)) = -\nabla p + \nabla \cdot \mu (\nabla u) + (\nabla u)^T )$
\pagebreak

$ N(u) = u \cdot \nabla u $
\pagebreak

$ N(u) = \nabla \cdot (u u) $
\pagebreak

$ \pi $
\pagebreak

$ Nx = [T M^{-1} T^{*}]x = b $
\pagebreak

$ x $
\pagebreak

$ M $
\pagebreak

$ [T M^{-1} T^{*}]^{-1} $
\pagebreak

$ Nx = b $
\pagebreak

$ Mx = [J L^{-1} S]x = b $
\pagebreak

$ Mx=b $
\pagebreak

$ Mx = b $
\pagebreak

$ F = \frac{\mathrm{d} \sigma}{\mathrm{d} T}(\nabla T |\nabla C| - (\nabla T \cdot \nabla \phi) \nabla C)$
\pagebreak

$\frac{\partial Q}{\partial \tau}+sgn(Q^0)(|\nabla Q | - 1) = 0$
\pagebreak

$\tilde{Q}$
\pagebreak

$Q = \tilde{Q} + \lambda_{ij}H'(Q^0)|\nabla Q^0|$
\pagebreak

$Q^0$
\pagebreak

$ (i,j,k,d):-> p $
\pagebreak

$ y $
\pagebreak

$ z $
\pagebreak

$ \frac{\partial \rho}{\partial t} + \nabla \cdot (\rho \mathbf{u}) = S(x,t) $
\pagebreak

$ \nabla \cdot (\rho \mathbf{u} \otimes \mathbf{u})$
\pagebreak

$ \nabla \cdot (\rho \mathbf{u} Q)$
\pagebreak

$ Q = C_\textrm{p} T$
\pagebreak

$ Q = h$
\pagebreak

$ m_\rho = \rho \mathbf{u} $
\pagebreak

$ \mathbf{u} $
\pagebreak

$ \nabla \cdot (\rho \mathbf{u} \otimes \mathbf{u}) = \nabla \cdot (m_\rho \otimes \mathbf{u} ) $
\pagebreak

$ \nabla \cdot (\rho \mathbf{u} Q) = \nabla \cdot (m_\rho Q) $
\pagebreak

$ L = C I + \nabla \cdot D \nabla$
\pagebreak

$ \mbox{$L u$} = \mbox{$(C I + \nabla \cdot D \nabla) u$} = f $
\pagebreak

\[ (C I + \nabla \cdot D \nabla) u = f \]
\pagebreak

$ C $
\pagebreak

$ D $
\pagebreak

$ f $
\pagebreak

$ u $
\pagebreak

$ -\nabla^2 u = f $
\pagebreak

$ (C I + \nabla \cdot D \nabla ) u = f $
\pagebreak

$C$
\pagebreak

$D$
\pagebreak

$u$
\pagebreak

$f$
\pagebreak

$ y=F[x] $
\pagebreak

$ z=F[x]+y $
\pagebreak

$z=F[x]+y$
\pagebreak

$F[x]=b$
\pagebreak

$ F'[x]v $
\pagebreak

$ y=Ax $
\pagebreak

$ z=Ax+y $
\pagebreak

$ y=A^{T} x $
\pagebreak

$ z=A^{T}x+y $
\pagebreak

$g$
\pagebreak

$y$
\pagebreak

$z$
\pagebreak

$ F[x]=b $
\pagebreak

$F[x]$
\pagebreak

$J[x] = F'[x]$
\pagebreak

$ \alpha $
\pagebreak

$ r_0 = r $
\pagebreak

$ r_1 = r_0 + 1 $
\pagebreak

$ L = \beta C I + \alpha \nabla \cdot \mu ( (\nabla u) + (\nabla u)^T ) $
\pagebreak

$ \mu $
\pagebreak

$ \mbox{$L u$} = C u + \nabla \cdot \mu (\nabla u + (\nabla u)^T) = f $
\pagebreak

\[ C u + \nabla \cdot \mu (\nabla u + (\nabla u)^T) = f \]
\pagebreak

$ \beta C u + \alpha \nabla \cdot \mu (\nabla u + (\nabla u)^T) = f $
\pagebreak

\end{document}
